fix Karatsuba's mult

code/experimental/rsa/Hacl.Impl.Multiplication.fst
@@ -68,6 +68,15 @@ val bn_mul:
 let bn_mul #aLen #bLen aaLen a bbLen b res = 
     bn_mult_ #aLen #bLen aaLen a bbLen b (size 0) (add #SIZE aaLen bbLen) res
 
+val bn_mul_u64:
+    #aLen:size_nat ->
+    aaLen:size_t{v aaLen == aLen /\ aLen + 1 < max_size_t} ->
+    a:lbignum aLen -> b:uint64 -> res:lbignum (aLen + 1) -> Stack unit
+    (requires (fun h -> live h a /\ live h res /\ disjoint res a))
+    (ensures (fun h0 _ h1 -> preserves_live h0 h1 /\ modifies1 res h0 h1))
+let bn_mul_u64 #aLen aaLen a b res = 
+    bn_mult_by_limb_addj #aLen aaLen a b (size 0) (size 0) (add #SIZE aaLen (size 1)) (u64 0) res
+
 val abs:
     #aLen:size_nat -> #bLen:size_nat ->
     aaLen:size_t{v aaLen == aLen} -> a:lbignum aLen ->
@@ -144,29 +153,55 @@ let rec karatsuba_ #aLen pow2_i iLen aaLen a b tmp res =
        let c0 = Buffer.sub #uint64 #(v aaLen2) #(2 * v pow2_i0) res (size 0) (mul #SIZE (size 2) pow2_i0) in
        karatsuba_ #(v pow2_i0) pow2_i0 (size 0) pow2_i0 a0 b0 tmp0 c0; // c0 = a0 * b0
 
-       let ind = if (pow2_i0 /. (size 2) <=. iLen) then sub #SIZE iLen (pow2_i0 /. (size 2)) else iLen in
-       let tmp0 = Buffer.sub #uint64 #(v tmpLen) #(4 * v pow2_i1) tmp (size 0) (mul #SIZE (size 4) pow2_i1) in
-       let c1 = Buffer.sub #uint64 #(v aaLen2) #(2 * v pow2_i1) res (mul #SIZE (size 2) pow2_i0) (mul #SIZE (size 2) pow2_i1) in
-       karatsuba_ #(v pow2_i1) pow2_i0 iLen pow2_i1 a1 b1 tmp0 c1; // c1 = a1 * b1
+       if (pow2_i1 =. size 1) then begin
+          let a1_0 = a1.(size 0) in
+          let b1_0 = b1.(size 0) in
+          let c1 = mul_wide a1_0 b1_0 in
+          let c1_0 = to_u64 #U128 c1 in
+          let c1_1 = to_u64 #U128 (shift_right #U128 c1 (u32 64)) in
+          let c0Len = mul #SIZE (size 2) pow2_i0 in
+          res.(c0Len) <- c1_0;
+          res.(add #SIZE c0Len (size 1)) <- c1_1;
+	  
+          let tmp0 = Buffer.sub #uint64 #(v tmpLen) #(v pow2_i0 + 1) tmp (size 0) (add #SIZE pow2_i0 (size 1)) in //tmp0 = a0 * b1_0
+          bn_mul_u64 #(v pow2_i0) pow2_i0 a0 b1_0 tmp0;
+          let tmp1 = Buffer.sub #uint64 #(v tmpLen) #(v pow2_i0 + 1) tmp (add #SIZE pow2_i0 (size 1)) (add #SIZE pow2_i0 (size 1)) in //tmp1 = b0 * a1_0
+          bn_mul_u64 #(v pow2_i0) pow2_i0 b0 a1_0 tmp1;
+          let tmp1Len = add #SIZE pow2_i0 (size 1) in
+          let tmp1Len2 = add #SIZE tmp1Len tmp1Len in
+          let tmp2Len = add #SIZE pow2_i0 (size 2) in
+          let tmp2 = Buffer.sub #uint64 #(v tmpLen) #(v tmp2Len) tmp tmp1Len2 tmp2Len in //tmp2 = tmp0 + tmp1 = a0 * b1_0 + b0 * a1_0
+          bn_add_carry #(v tmp1Len) #(v tmp1Len) tmp1Len tmp0 tmp1Len tmp1 tmp2;
+	  
+          let res1Len = add #SIZE pow2_i0 (size 2) in
+          let res1 = Buffer.sub #uint64 #(v aaLen2) #(v res1Len) res pow2_i0 res1Len in
+          bn_add res1Len res1 tmp2Len tmp2 res1 //FIXME!!!
+          end 
+       else begin
+          let ind = if (pow2_i0 /. (size 2) <=. iLen) then sub #SIZE iLen (pow2_i0 /. (size 2)) else iLen in
+          let tmp0 = Buffer.sub #uint64 #(v tmpLen) #(4 * v pow2_i1) tmp (size 0) (mul #SIZE (size 4) pow2_i1) in
+          let c1 = Buffer.sub #uint64 #(v aaLen2) #(2 * v pow2_i1) res (mul #SIZE (size 2) pow2_i0) (mul #SIZE (size 2) pow2_i1) in
+          karatsuba_ #(v pow2_i1) pow2_i0 iLen pow2_i1 a1 b1 tmp0 c1; // c1 = a1 * b1
 	    
-       let a2 = Buffer.sub #uint64 #(v tmpLen) #(v pow2_i0) tmp (size 0) pow2_i0 in
-       let b2 = Buffer.sub #uint64 #(v tmpLen) #(v pow2_i0) tmp pow2_i0 pow2_i0 in
-       abs #(v pow2_i0) #(v pow2_i1) pow2_i0 a0 pow2_i1 a1 a2; // a2 = |a0 - a1|
-       abs #(v pow2_i0) #(v pow2_i1) pow2_i0 b0 pow2_i1 b1 b2; // b2 = |b0 - b1|
+          let a2 = Buffer.sub #uint64 #(v tmpLen) #(v pow2_i0) tmp (size 0) pow2_i0 in
+          let b2 = Buffer.sub #uint64 #(v tmpLen) #(v pow2_i0) tmp pow2_i0 pow2_i0 in
+          abs #(v pow2_i0) #(v pow2_i1) pow2_i0 a0 pow2_i1 a1 a2; // a2 = |a0 - a1|
+          abs #(v pow2_i0) #(v pow2_i1) pow2_i0 b0 pow2_i1 b1 b2; // b2 = |b0 - b1|
 
-       let c2 = Buffer.sub #uint64 #(v aaLen2) #(2 * v pow2_i0) tmp (mul #SIZE (size 2) pow2_i0) (mul #SIZE (size 2) pow2_i0) in
-       let tmp0 = Buffer.sub #uint64 #(v tmpLen) #(4 * v pow2_i0) tmp (mul #SIZE (size 4) pow2_i0) (mul #SIZE (size 4) pow2_i0) in
-       karatsuba_ #(v pow2_i0) pow2_i0 (size 0) pow2_i0 a2 b2 tmp0 c2; // c2 = a2 * b2
+          let c2 = Buffer.sub #uint64 #(v aaLen2) #(2 * v pow2_i0) tmp (mul #SIZE (size 2) pow2_i0) (mul #SIZE (size 2) pow2_i0) in
+          let tmp0 = Buffer.sub #uint64 #(v tmpLen) #(4 * v pow2_i0) tmp (mul #SIZE (size 4) pow2_i0) (mul #SIZE (size 4) pow2_i0) in
+          karatsuba_ #(v pow2_i0) pow2_i0 (size 0) pow2_i0 a2 b2 tmp0 c2; // c2 = a2 * b2
 
-       let tmp1Len = add #SIZE pow2_i (size 1) in
-       let tmp1 = Buffer.sub #uint64 #(v tmpLen) #(v tmp1Len) tmp (mul #SIZE (size 4) pow2_i0) tmp1Len in
-       add_sign #(v pow2_i0) #(v pow2_i1) #(v tmp1Len) pow2_i0 pow2_i1 tmp1Len c0 c1 c2 a0 a1 a2 b0 b1 b2 tmp1; //tmp1 = (c0 + c1) +/- c2
+          let tmp1Len = add #SIZE pow2_i (size 1) in
+          let tmp1 = Buffer.sub #uint64 #(v tmpLen) #(v tmp1Len) tmp (mul #SIZE (size 4) pow2_i0) tmp1Len in
+          add_sign #(v pow2_i0) #(v pow2_i1) #(v tmp1Len) pow2_i0 pow2_i1 tmp1Len c0 c1 c2 a0 a1 a2 b0 b1 b2 tmp1; //tmp1 = (c0 + c1) +/- c2
 
-       //res = [c0; c1]
-       //tmp = [a2; b2; c2; tmp1; _]
-       let res1Len = add #SIZE pow2_i0 (add #SIZE pow2_i1 pow2_i1) in
-       let res1 = Buffer.sub #uint64 #(v aaLen2) #(v res1Len) res pow2_i0 res1Len in
-       bn_add res1Len res1 tmp1Len tmp1 res1 //FIXME!!!
+          //res = [c0; c1]
+          //tmp = [a2; b2; c2; tmp1; _]
+          let res1Len = add #SIZE pow2_i0 (add #SIZE pow2_i1 pow2_i1) in
+          let res1 = Buffer.sub #uint64 #(v aaLen2) #(v res1Len) res pow2_i0 res1Len in
+          bn_add res1Len res1 tmp1Len tmp1 res1 //FIXME!!!
+          end
     end
 
 // aLen + iLen == pow2_i
